proof/refine/ARM_HYP/ArchInvsDefs_H.thy
@@ -151,6 +151,12 @@ definition valid_arch_cap' :: "arch_capability \<Rightarrow> kernel_state \<Righ
 lemmas valid_arch_cap'_simps[simp] =
   valid_arch_cap'_def[split_simps arch_capability.split, simplified]
 
+definition arch_valid_irq :: "irq \<Rightarrow> bool" where
+  "arch_valid_irq irq \<equiv> irq \<le> maxIRQ"
+
+(* within the Arch locale, we want automatic expansion of the valid irq conditions *)
+lemmas [simp] = arch_valid_irq_def
+
 definition valid_arch_tcb' :: "Structures_H.arch_tcb \<Rightarrow> kernel_state \<Rightarrow> bool" where
   "valid_arch_tcb' \<equiv> \<lambda>t s. \<forall>v. atcbVCPUPtr t = Some v \<longrightarrow> vcpu_at' v s "
 
